src/ObviousDisequality.v
@@ -1,17 +1,15 @@
-Add LoadPath "~/JB/minikanren-coq/src/".
-
 Require Import List.
 Import ListNotations.
 (*Require Import Coq.Lists.ListSet.*)
 Require Import Extraction.
 
 Require Import Unify.
-Require Import MiniKanrenSyntaxDiseq.
+Require Import MiniKanrenSyntax.
 Require Import Stream.
-Require Import DenotationalSemDiseq.
-Require Import OperationalSemDiseq.
-Require Import OpSemDiseqSoundness.
-Require Import OpSemCompletenessDiseq.
+Require Import DenotationalSem.
+Require Import OperationalSem.
+Require Import OpSemSoundness.
+Require Import OpSemCompleteness.
 
 
 Module ObviousConstraintStore <: ConstraintStoreSig.
@@ -20,8 +18,10 @@ Definition constraint_store (s : subst) : Set := list (term * term).
 
 Definition init_cs : constraint_store empty_subst := [].
 
-Inductive add_constraint : forall (s : subst), constraint_store s -> term -> term -> option (constraint_store s) -> Set :=
-| acC : forall s cs t1 t2, add_constraint s cs t1 t2 (Some ((t1, t2) :: cs)).
+Inductive add_constraint_ind_def : forall (s : subst), constraint_store s -> term -> term -> option (constraint_store s) -> Set :=
+| acC : forall s cs t1 t2, add_constraint_ind_def s cs t1 t2 (Some ((t1, t2) :: cs)).
+
+Definition add_constraint := add_constraint_ind_def.
 
 Lemma add_constraint_exists :
   forall (s : subst) (cs : constraint_store s) (t1 t2 : term),
@@ -31,100 +31,80 @@ Proof. intros. eexists. econstructor. Qed.
 Lemma add_constraint_unique :
   forall (s : subst) (cs : constraint_store s) (t1 t2 : term) (r r' : option (constraint_store s)),
     add_constraint s cs t1 t2 r -> add_constraint s cs t1 t2 r' -> r = r'.
-Proof. intros. good_inversion H. good_inversion H0. simpl_existT_cs_same.
+Proof. intros. good_inversion H. good_inversion H0. simpl_existT_cs_same. reflexivity. Qed.
 
-Parameter upd_cs : forall (s : subst), constraint_store s -> forall (d : subst), option (constraint_store (compose s d)) -> Set.
+Inductive upd_cs_ind_def : forall (s : subst), constraint_store s -> forall (d : subst), option (constraint_store (compose s d)) -> Set :=
+| uC : forall s cs d, upd_cs_ind_def s cs d (Some cs).
 
-Parameter upd_cs_exists :
+Definition upd_cs := upd_cs_ind_def.
+
+Lemma upd_cs_exists :
   forall (s : subst) (cs : constraint_store s) (d : subst),
     {r : option (constraint_store (compose s d)) & upd_cs s cs d r}.
+Proof. intros. eexists. econstructor. Qed.
 
-Parameter upd_cs_unique :
+Lemma upd_cs_unique :
   forall (s : subst) (cs : constraint_store s) (d : subst) (r r' : option (constraint_store (compose s d))),
     upd_cs s cs d r -> upd_cs s cs d r' -> r = r'.
+Proof. intros. good_inversion H. good_inversion H0. simpl_existT_cs_same. reflexivity. Qed.
 
-Parameter in_denotational_sem_cs : forall (s : subst), constraint_store s -> repr_fun -> Prop.
+Definition in_denotational_sem_cs (s : subst) (cs : constraint_store s) (f : repr_fun) :=
+  forall (t1 t2 : term), In (t1, t2) cs -> ~ gt_eq (apply_repr_fun f t1) (apply_repr_fun f t2).
 
 Notation "[| s , cs , f |]" := (in_denotational_sem_cs s cs f) (at level 0).
 
-Axiom init_condition : forall f, [| empty_subst , init_cs , f |].
+Lemma init_condition : forall f, [| empty_subst , init_cs , f |].
+Proof. unfold in_denotational_sem_cs. contradiction. Qed.
 
-Axiom add_constraint_fail_condition :
+Lemma add_constraint_fail_condition :
   forall (s : subst) (cs : constraint_store s) (t1 t2 : term),
     add_constraint s cs t1 t2 None ->
-    forall f, ~ ([| s , cs  , f |] /\ [ s , f ] /\ (~ gt_eq (apply_repr_fun f t1) (apply_repr_fun f t2))).
+    forall f, ~ ([| s , cs  , f |] /\ [ s , f ] /\ [| Disunify t1 t2 , f |]).
+Proof. intros. inversion H. Qed.
 
-Axiom add_constraint_success_condition :
+Lemma add_constraint_success_condition :
   forall (s : subst) (cs cs' : constraint_store s) (t1 t2 : term),
     add_constraint s cs t1 t2 (Some cs') ->
     forall f, [| s , cs' , f |] /\ [ s , f ] <->
-              [| s , cs  , f |] /\ [ s , f ] /\ (~ gt_eq (apply_repr_fun f t1) (apply_repr_fun f t2)).
+              [| s , cs  , f |] /\ [ s , f ] /\ [| Disunify t1 t2 , f |].
+Proof.
+  unfold in_denotational_sem_cs. intros.
+  good_inversion H. simpl_existT_cs_same. good_inversion H4. split.
+  { intros [DSCS DSS]. split; try split; intros; auto.
+    { apply DSCS. right. auto. }
+    { constructor. apply DSCS. left. auto. }  }
+  { intros [DSCS [DSS DSG]]. good_inversion DSG. split; auto. intros.
+    destruct H; auto. good_inversion H; auto. }
+Qed.
 
-Axiom upd_cs_fail_condition :
+Lemma upd_cs_fail_condition :
   forall (s : subst) (cs : constraint_store s) (d : subst),
     upd_cs s cs d None -> forall f, ~ ([| s , cs , f |] /\ [ compose s d , f ]).
+Proof. intros. inversion H. Qed.
 
-Axiom upd_cs_success_condition :
+Lemma upd_cs_success_condition :
   forall (s : subst) (cs : constraint_store s) (d : subst) (cs' : constraint_store (compose s d)),
     upd_cs s cs d (Some cs') ->
     forall f, [| compose s d , cs' , f |] /\ [ compose s d , f ] <->
               [| s           , cs  , f |] /\ [ compose s d , f ].
+Proof.
+  unfold in_denotational_sem_cs. intros. good_inversion H. simpl_existT_cs_same.
+  good_inversion H3. reflexivity.
+Qed.
 
 End ObviousConstraintStore.
 
 
+Module OperationalSemObviousCS := OperationalSemAbstr ObviousConstraintStore.
 
-Module Type ConstraintStoreSig.
+Module OperationalSemObviousCSSoundness := OperationalSemSoundnessAbstr ObviousConstraintStore.
 
-Parameter constraint_store : subst -> Set.
+Module OperationalSemObviousCSCompleteness := OperationalSemCompletenessAbstr ObviousConstraintStore.
 
-Parameter init_cs : constraint_store empty_subst.
+Import OperationalSemObviousCS.
 
-Parameter add_constraint : forall (s : subst), constraint_store s -> term -> term -> option (constraint_store s) -> Set.
+Extraction Language Haskell.
 
-Parameter add_constraint_exists :
-  forall (s : subst) (cs : constraint_store s) (t1 t2 : term),
-    {r : option (constraint_store s) & add_constraint s cs t1 t2 r}.
+Extraction "extracted/obvious_diseq_interpreter.hs" op_sem_exists.
 
-Parameter add_constraint_unique :
-  forall (s : subst) (cs : constraint_store s) (t1 t2 : term) (r r' : option (constraint_store s)),
-    add_constraint s cs t1 t2 r -> add_constraint s cs t1 t2 r' -> r = r'.
 
-Parameter upd_cs : forall (s : subst), constraint_store s -> forall (d : subst), option (constraint_store (compose s d)) -> Set.
-
-Parameter upd_cs_exists :
-  forall (s : subst) (cs : constraint_store s) (d : subst),
-    {r : option (constraint_store (compose s d)) & upd_cs s cs d r}.
-
-Parameter upd_cs_unique :
-  forall (s : subst) (cs : constraint_store s) (d : subst) (r r' : option (constraint_store (compose s d))),
-    upd_cs s cs d r -> upd_cs s cs d r' -> r = r'.
-
-Parameter in_denotational_sem_cs : forall (s : subst), constraint_store s -> repr_fun -> Prop.
-
-Notation "[| s , cs , f |]" := (in_denotational_sem_cs s cs f) (at level 0).
-
-Axiom init_condition : forall f, [| empty_subst , init_cs , f |].
-
-Axiom add_constraint_fail_condition :
-  forall (s : subst) (cs : constraint_store s) (t1 t2 : term),
-    add_constraint s cs t1 t2 None ->
-    forall f, ~ ([| s , cs  , f |] /\ [ s , f ] /\ (~ gt_eq (apply_repr_fun f t1) (apply_repr_fun f t2))).
-
-Axiom add_constraint_success_condition :
-  forall (s : subst) (cs cs' : constraint_store s) (t1 t2 : term),
-    add_constraint s cs t1 t2 (Some cs') ->
-    forall f, [| s , cs' , f |] /\ [ s , f ] <->
-              [| s , cs  , f |] /\ [ s , f ] /\ (~ gt_eq (apply_repr_fun f t1) (apply_repr_fun f t2)).
-
-Axiom upd_cs_fail_condition :
-  forall (s : subst) (cs : constraint_store s) (d : subst),
-    upd_cs s cs d None -> forall f, ~ ([| s , cs , f |] /\ [ compose s d , f ]).
-
-Axiom upd_cs_success_condition :
-  forall (s : subst) (cs : constraint_store s) (d : subst) (cs' : constraint_store (compose s d)),
-    upd_cs s cs d (Some cs') ->
-    forall f, [| compose s d , cs' , f |] /\ [ compose s d , f ] <->
-              [| s           , cs  , f |] /\ [ compose s d , f ].
-
-End ConstraintStoreSig.
