src/OpSemCompleteness.v
@@ -1,284 +1,169 @@
 Require Import List.
 Require Import Coq.Lists.ListSet.
-Import ListNotations.
+Require Import Omega.
+
 Require Import Stream.
 Require Import Unify.
 Require Import MiniKanrenSyntax.
 Require Import OperationalSem.
 Require Import DenotationalSem.
-Require Import Omega.
-
-Definition in_denotational_sem_subst (s : subst) (f : repr_fun) : Prop :=
-  exists (f' : repr_fun), repr_fun_eq (subst_repr_fun_compose s f') f.
 
 
-Definition in_denotational_analog (t : trace) (f : repr_fun) : Prop :=
-  exists (s : subst) (n : nat), in_stream (Answer s n) t /\ in_denotational_sem_subst s f.
+Module OperationalSemCompletenessAbstr (CS : ConstraintStoreSig).
 
-Notation "{| t , f |}" := (in_denotational_analog t f).
+Import CS.
 
-Lemma set_empty_union
-      (s1 s2 : var_set)
-      (EQ : var_set_union s1 s2 = var_set_empty) :
-      s1 = var_set_empty /\ s2 = var_set_empty.
-Proof.
-  split.
-  { destruct s1; auto.
-    assert (In n var_set_empty).
-    { rewrite <- EQ. apply set_union_intro. left. constructor. auto. }
-    inversion H. }
-  { destruct s2; auto.
-    assert (In n var_set_empty).
-    { rewrite <- EQ. apply set_union_intro. right. constructor. auto. }
-    inversion H. }
-Qed.
+Module OperationalSemCS := OperationalSemAbstr CS.
 
-Lemma unfier_from_gt_unifier
-      (t1 t2 : term)
-      (f : repr_fun)
-      (F_UNIFIES : gt_eq (apply_repr_fun f t1) (apply_repr_fun f t2)) :
-      exists s, unifier s t1 t2 /\ in_denotational_sem_subst s f.
-Proof.
-  remember (map (fun x => (x, proj1_sig (f x))) (var_set_union (fv_term t1) (fv_term t2))) as s.
-  exists s. split.
-  { red. red in F_UNIFIES.
-    assert (apply_subst s t1 = proj1_sig (apply_repr_fun f t1)).
-    { clear F_UNIFIES.
-      assert (forall x, In x (fv_term t1) -> image s x = Some (proj1_sig (f x))).
-      { intros. assert (In x (var_set_union (fv_term t1) (fv_term t2))).
-        { apply set_union_intro1. auto. }
-        remember (var_set_union (fv_term t1) (fv_term t2)).
-        subst. apply map_image. auto. }
-      apply subst_of_gt. auto. }
-    assert (apply_subst s t2 = proj1_sig (apply_repr_fun f t2)).
-    { clear F_UNIFIES.
-      assert (forall x, In x (fv_term t2) -> image s x = Some (proj1_sig (f x))).
-      { intros. assert (In x (var_set_union (fv_term t1) (fv_term t2))).
-        { apply set_union_intro2. auto. }
-        remember (var_set_union (fv_term t1) (fv_term t2)).
-        subst. apply map_image. auto. }
-      apply subst_of_gt. auto. }
-    congruence. }
-  { red. exists f. red. intros x. unfold subst_repr_fun_compose.
-    unfold apply_subst. destruct (image s x) eqn:eq.
-    { destruct (f x) eqn:eqfx.
-      assert (x0 = t).
-      { unfold image in eq.
-        remember (var_set_union (fv_term t1) (fv_term t2)). clear Heqv.
-        revert Heqs. revert v.
-        induction s.
-        { inversion eq. }
-        { intros. destruct a as [y t0]. destruct v; good_inversion Heqs.
-          destruct (Nat.eq_dec n x).
-          { good_inversion eq. rewrite eqfx. auto. }
-          { apply IHs with v; auto. } } }
-      subst. red. simpl. clear eqfx. clear eq. induction t.
-      { inversion e. }
-      { auto. }
-      { simpl in e. apply set_empty_union in e. destruct e.
-        apply IHt1 in H. apply IHt2 in H0. simpl.
-        destruct (apply_repr_fun f t3). simpl in H.
-        destruct (apply_repr_fun f t4). simpl in H0.
-        simpl. subst. auto. } }
-    { red. auto. } }
-Qed.
+Import OperationalSemCS.
 
 Lemma search_completeness_generalized
-      (l     : nat)
-      (g     : goal)
-      (CG    : consistent_goal g)
-      (s     : subst)
-      (n     : nat)
-      (WF : well_formed_state' (Leaf g s n))
-      (t     : trace)
-      (OP   : op_sem (State (Leaf g s n)) t)
-      (f     : repr_fun)
-      (DSG : [| l | g , f |])
-      (DSS : in_denotational_sem_subst s f) :
+      (l    : nat)
+      (g    : goal)
+      (CG   : consistent_goal g)
+      (s    : subst)
+      (cs   : constraint_store s)
+      (n    : nat)
+      (WF   : well_formed_state' (Leaf g s cs n))
+      (t    : trace)
+      (OP   : op_sem (State (Leaf g s cs n)) t)
+      (f    : repr_fun)
+      (DSG  : [| l | g , f |])
+      (DSS  : [ s , f ])
+      (DSCS : [| s , cs , f |]) :
       exists (f' : repr_fun), {| t , f' |} /\
                             forall (x : name), x < n -> gt_eq (f x) (f' x).
 Proof.
-  revert OP. revert t. revert CG DSG DSS WF. revert g f s n. induction l.
+  revert OP. revert t. revert CG DSG DSS DSCS WF. revert cs. revert g f s n. induction l.
   { intros. apply in_denotational_sem_zero_lev in DSG. contradiction. }
   { induction g; intros; good_inversion CG.
     { good_inversion DSG. }
     { exists f. split.
-      { econstructor; eexists; split; eauto.
-        good_inversion OP. good_inversion EV. constructor. }
+      { econstructor. eexists. eexists. split; eauto.
+        good_inversion OP. good_inversion EV. simpl_existT_cs_same. constructor. }
       { intros; red; auto. } }
     { exists f. split.
       2: intros; red; auto.
-      good_inversion DSG. red in DSS. destruct DSS as [fs s_fs_f].
-      assert (gt_eq (apply_repr_fun fs (apply_subst s t)) (apply_repr_fun fs (apply_subst s t0))).
-      { red. rewrite <- repr_fun_apply_compose. rewrite <- repr_fun_apply_compose.
-        apply eq_trans with (proj1_sig (apply_repr_fun f t)).
-        { apply repr_fun_eq_apply. auto. }
-        { apply eq_trans with (proj1_sig (apply_repr_fun f t0)); auto.
-          symmetry. apply repr_fun_eq_apply. auto. } }
-      apply unfier_from_gt_unifier in H. destruct H as [u [u_uni u_fs]].
-      good_inversion OP. good_inversion EV.
-      { specialize (mgu_non_unifiable _ _ MGU u u_uni). contradiction. }
-      { rename s' into m. red. exists (compose s m). exists n. split; try constructor.
-        specialize (mgu_most_general _ _ _ u MGU u_uni). intro Hmg.
-        red in Hmg. destruct Hmg as [ds u_ds_m]. red in u_fs.
-        destruct u_fs as [fss u_fss_fs]. red. exists (subst_repr_fun_compose ds fss).
-        eapply repr_fun_eq_trans. 2: eauto.
-        eapply repr_fun_eq_trans. eapply subst_repr_fun_compose_assoc_subst.
-        eapply repr_fun_eq_trans. 2: eapply repr_fun_eq_compose; eauto.
-        apply repr_fun_eq_compose.
-        eapply repr_fun_eq_trans. red; symmetry; eapply subst_repr_fun_compose_assoc_subst.
-        apply repr_fun_compose_eq. intros. rewrite u_ds_m. apply compose_correctness. } }
+      good_inversion OP. good_inversion EV; good_inversion DSG; simpl_existT_cs_same.
+      { destruct DSS as [fs COMP_s_fs]. red in UNI.
+        rewrite <- (repr_fun_eq_apply _ _ t COMP_s_fs) in UNI.
+        rewrite <- (repr_fun_eq_apply _ _ t0 COMP_s_fs) in UNI.
+        rewrite (repr_fun_apply_compose s fs t) in UNI.
+        rewrite (repr_fun_apply_compose s fs t0) in UNI.
+        apply unfier_from_gt_unifier in UNI.
+        destruct UNI as [sc [SC_UNIFIES _]]. specialize (mgu_non_unifiable _ _ MGU sc).
+        contradiction. }
+      { specialize (upd_cs_fail_condition _ _ _ UPD_CS f).
+        intros C. exfalso. apply C. split; auto.
+        apply (denotational_sem_uni _ _ _ _ MGU); auto. }
+      { red. exists (compose s d). exists cs'. exists n. split.
+        { constructor. }
+        { apply and_comm. specialize (upd_cs_success_condition _ _ _ _ UPD_CS f).
+          intro EQUI. apply EQUI. split; auto. apply (denotational_sem_uni _ _ _ _ MGU); auto. } } }
+    { exists f. split.
+      2: intros; red; auto.
+      good_inversion DSG. good_inversion OP.
+      good_inversion EV; simpl_existT_cs_same.
+      { exfalso. eapply add_constraint_fail_condition in ADD_C. eauto. }
+      { red. exists s. exists cs'. exists n. split.
+        { constructor. }
+        { apply and_comm. eapply add_constraint_success_condition in ADD_C.
+          apply ADD_C. auto. } } }
     { good_inversion OP. inversion EV; subst.
-      apply well_formedness_preservation in EV; auto. good_inversion EV.
+      apply well_formedness_preservation in EV; auto. good_inversion EV. simpl_existT_cs_same.
       good_inversion wfState.
-      specialize (op_sem_exists (State (Leaf g1 s n))). intro p1. destruct p1 as [t1 OP1].
-      specialize (op_sem_exists (State (Leaf g2 s n))). intro p2. destruct p2 as [t2 OP2].
+      specialize (op_sem_exists (State (Leaf g1 s cs n))). intro p1. destruct p1 as [t1 OP1].
+      specialize (op_sem_exists (State (Leaf g2 s cs n))). intro p2. destruct p2 as [t2 OP2].
       specialize (sum_op_sem _ _ _ _ _ OP1 OP2 OP0). intro Hinter.
       good_inversion DSG.
-      { specialize (IHg1 f s n CG_G1 DSG0 DSS WF_L t1 OP1).
+      { specialize (IHg1 f s n cs CG_G1 DSG0 DSS DSCS WF_L t1 OP1).
         destruct IHg1 as [f' [HinDA ff'_eq]]. exists f'. split; auto.
-        red in HinDA. destruct HinDA as [sr [nr [Hin DSSr]]].
-        red. exists sr. exists nr. split; auto. constructor.
-        apply (interleave_in _ _ _ Hinter (Answer sr nr)). auto. }
-      { specialize (IHg2 f s n CG_G2 DSG0 DSS WF_R t2 OP2).
+        red in HinDA. destruct HinDA as [sr [csr [nr [Hin [DSSr DSCSr]]]]].
+        red. exists sr. exists csr. exists nr. split; auto. constructor.
+        apply (interleave_in _ _ _ Hinter (Answer sr csr nr)). auto. }
+      { specialize (IHg2 f s n cs CG_G2 DSG0 DSS DSCS WF_R t2 OP2).
         destruct IHg2 as [f' [HinDA ff'_eq]]. exists f'. split; auto.
-        red in HinDA. destruct HinDA as [sr [nr [Hin DSSr]]].
-        red. exists sr. exists nr. split; auto. constructor.
-        apply (interleave_in _ _ _ Hinter (Answer sr nr)). auto. } }
-    { good_inversion DSG. good_inversion OP. inversion EV; subst.
-      specialize (op_sem_exists (State (Leaf g1 s n))). intro p1. destruct p1 as [t1 OP1].
-      assert (wfst'1 : well_formed_state' (Leaf g1 s n)).
-      { constructor; good_inversion WF; auto. }
-      specialize (IHg1 f s n CG_G1 DSG_L DSS wfst'1 t1 OP1).
+        red in HinDA. destruct HinDA as [sr [csr [nr [Hin [DSSr DSCSr]]]]].
+        red. exists sr. exists csr. exists nr. split; auto. constructor.
+        apply (interleave_in _ _ _ Hinter (Answer sr csr nr)). auto. } }
+    { good_inversion DSG. good_inversion OP. inversion EV; simpl_existT_cs_same; subst.
+      specialize (op_sem_exists (State (Leaf g1 s cs n))). intro p1. destruct p1 as [t1 OP1].
+      assert (wfst'1 : well_formed_state' (Leaf g1 s cs n)).
+      { constructor; good_inversion WF; simpl_existT_cs_same; auto. }
+      specialize (IHg1 f s n cs CG_G1 DSG_L DSS DSCS wfst'1 t1 OP1).
       destruct IHg1 as [f' [HinDA ff'_eq]]. red in HinDA.
-      destruct HinDA as [s' [n' [Hinstr' HDAS']]].
-      specialize (op_sem_exists (State (Leaf g2 s' n'))). intro p2. destruct p2 as [t2 OP2].
-      specialize (counter_in_trace _ _ _ _ _ _ OP1 Hinstr'). intro n_le_n'.
-      assert (wfst'2 : well_formed_state' (Leaf g2 s' n')).
-      { good_inversion WF.
-        specialize (well_formed_subst_in_trace _ (wfNonEmpty _ wfst'1)  _ OP1 _ _ Hinstr').
-        intros. destruct H.
-        constructor; auto. intros.
+      destruct HinDA as [s' [cs' [n' [Hinstr' [HDAS' HDACS']]]]].
+      specialize (op_sem_exists (State (Leaf g2 s' cs' n'))). intro p2. destruct p2 as [t2 OP2].
+      specialize (counter_in_trace _ _ _ _ _ _ _ _ OP1 Hinstr'). intro n_le_n'.
+      assert (wfst'2 : well_formed_state' (Leaf g2 s' cs' n')).
+      { good_inversion WF. simpl_existT_cs_same.
+        destruct (well_formed_subst_in_trace _ (wfNonEmpty _ wfst'1)  _ OP1 _ _ _ Hinstr').
+        specialize (well_formed_ds_in_trace _ (wfNonEmpty _ wfst'1)  _ OP1 _ _ _ Hinstr').
+        intros. constructor; auto. intros.
         apply lt_le_trans with n; auto. }
       assert (Hg2' : in_denotational_sem_lev_goal (S l) g2 f').
       { apply completeness_condition_lev with f; auto. intros. apply ff'_eq.
         good_inversion WF. auto. }
-      specialize (IHg2 f' s' n' CG_G2 Hg2' HDAS' wfst'2 t2 OP2).
+      specialize (IHg2 f' s' n' cs' CG_G2 Hg2' HDAS' HDACS' wfst'2 t2 OP2).
       destruct IHg2 as [f'' [HinDA f'f''_eq]]. red in HinDA.
-      destruct HinDA as [s'' [n'' [Hinstr'' HDAS'']]].
+      destruct HinDA as [s'' [cs'' [n'' [Hinstr'' [HDAS'' HDACS'']]]]].
       exists f''. split.
-      { red. exists s''. exists n''. split; auto.
+      { red. exists s''. exists cs''. exists n''. split; auto.
         constructor. eapply prod_op_sem_in; eauto. }
       { intros. red. apply eq_trans with (proj1_sig (f' x)).
         { apply ff'_eq. auto. }
         { apply f'f''_eq. omega. } } }
-    { good_inversion DSG. good_inversion OP. inversion EV; subst.
+    { good_inversion DSG. good_inversion OP. inversion EV; simpl_existT_cs_same; subst.
       apply well_formedness_preservation in EV; auto. good_inversion EV.
       rename fn into fa.
-      red in DSS. destruct DSS as [fs fssf'_eq].
       remember (fun x => if name_eq_dec x n
                          then fa a
-                         else fs x) as fs'.
-      remember (fun x => if name_eq_dec x n
-                         then fa a
-                         else if name_eq_dec x a
-                              then (subst_repr_fun_compose s fs') a
-                              else fa x) as fn.
-      assert (H_n_is_fresh : forall x, In n (fv_term (apply_subst s (Var x))) -> x = n).
-      { intros. simpl in H0.
-        destruct (image s x) eqn:eq.
-        { assert (n < n).
-          { good_inversion WF. apply VRAN_LT_COUNTER.
-            red. eauto. }
-          omega. }
-        { simpl in H0. destruct H0; try contradiction. auto. } }
-      assert (Hgn : in_denotational_sem_lev_goal (S l) (g n) fn).
-      { rewrite Heqfn. good_inversion WF.
-        apply den_sem_another_fresh_var with n a fa; auto.
+                         else f x) as fn.
+      assert (Hgn : [| S l | g n , fn |]).
+      { good_inversion WF. apply den_sem_another_fresh_var with n a fa; auto.
         { intro C. apply FV_LT_COUNTER in C. omega. }
-        { destruct (name_eq_dec n n); try contradiction. reflexivity. }
-        { intros. destruct (name_eq_dec x n); try contradiction.
-          destruct (name_eq_dec x a); try contradiction. reflexivity. } }
-      assert (DSSn: in_denotational_sem_subst s fn).
-      { red. exists fs'. red. intros. red. unfold subst_repr_fun_compose.
-        rewrite Heqfs'. rewrite Heqfn. destruct (name_eq_dec x n).
-        { assert (H_n_is_fresh_2 : apply_subst s (Var n) = Var n).
-          { simpl. destruct (image s n) eqn:eq; auto.
-            good_inversion WF. assert (n < n).
-            { apply DOM_LT_COUNTER. red. eauto. }
-            omega. }
-          rewrite e. rewrite H_n_is_fresh_2. simpl.
-          destruct (name_eq_dec n n); try contradiction. auto. }
-        { destruct (name_eq_dec x a).
-          { rewrite e. rewrite Heqfs'. auto. }
-          { specialize (EASE x n1). rewrite EASE.
-            red in fssf'_eq. specialize (fssf'_eq x). red in fssf'_eq.
-            rewrite <- fssf'_eq. unfold subst_repr_fun_compose.
-            apply apply_repr_fun_fv. intros. destruct (name_eq_dec x0 n).
-            { rewrite e in H0. apply H_n_is_fresh in H0. contradiction. }
-            { reflexivity. } } } }
-      specialize (H n fn s (S n) (CG_BODY n) Hgn DSSn wfState t0 OP0).
+        {  destruct (name_eq_dec n n); try contradiction. reflexivity. }
+        { intros. destruct (name_eq_dec x n); try contradiction. auto. } }
+      assert (DSSn_AND_DSCSn : [ s , fn ] /\ [| s , cs , fn |]).
+      { good_inversion WF. simpl_existT_cs_same. apply (DS_LT_COUNTER f); auto.
+        intros. destruct (name_eq_dec x n); try omega. reflexivity. }
+      destruct DSSn_AND_DSCSn as [DSSn DSCSn].
+      specialize (H n fn s (S n) cs (CG_BODY n) Hgn DSSn DSCSn wfState t0 OP0).
       destruct H as [f' [HinDA ff'_eq]]. exists f'. split.
-      { red. red in HinDA. destruct HinDA as [s' [n' [Hinstr HDAS]]].
-        exists s'. exists n'. split; auto. constructor; auto. }
+      { red. red in HinDA. destruct HinDA as [s' [cs' [n' [Hinstr [HDAS HDACS]]]]].
+        exists s'. exists cs'. exists n'. split; auto. constructor; auto. }
       { intros. assert (x < S n). { omega. }
         specialize (ff'_eq x H0). red in ff'_eq. red. rewrite <- ff'_eq.
-        rewrite Heqfn. destruct (name_eq_dec x n); try omega.
-        destruct (name_eq_dec x a).
-        { rewrite e.
-          red in fssf'_eq. specialize (fssf'_eq a). red in fssf'_eq.
-          rewrite <- fssf'_eq. unfold subst_repr_fun_compose.
-          apply apply_repr_fun_fv. intros. rewrite Heqfs'.
-          destruct (name_eq_dec x0 n).
-          { auto. rewrite e0 in H1. apply H_n_is_fresh in H1. subst. contradiction. }
-          { unfold gt_eq. auto. } }
-        { specialize (EASE x n1). rewrite EASE. auto. } } }
+        rewrite Heqfn. destruct (name_eq_dec x n); try omega. reflexivity. } }
     { good_inversion DSG. good_inversion OP. inversion EV; subst.
-      apply well_formedness_preservation in EV; auto. good_inversion EV.
+      apply well_formedness_preservation in EV; auto. good_inversion EV. simpl_existT_cs_same.
       assert (cg_body : consistent_goal (proj1_sig (MiniKanrenSyntax.Prog n) t)).
       { remember (MiniKanrenSyntax.Prog n) as d. destruct d as [rel [Hcl Hco]].
         red in Hco. destruct (Hco t) as [Hcog Hcof]. auto. }
-      specialize (IHl (proj1_sig (MiniKanrenSyntax.Prog n) t) f s n0 cg_body DSG0 DSS wfState t1 OP0).
+      specialize (IHl (proj1_sig (MiniKanrenSyntax.Prog n) t) f s n0 cs cg_body DSG0 DSS DSCS wfState t1 OP0).
       destruct IHl as [f' [HinDA ff'_eq]]. exists f'. split; auto.
-      red. red in HinDA. destruct HinDA as [s' [n' [Hinstr HDAS]]].
-      exists s'. exists n'. split; auto. constructor; auto. } }
-Qed.
-
-Fixpoint first_nats (k : nat) : list nat :=
-  match k with
-  | 0   => []
-  | S n => n :: first_nats n
-  end.
-
-Lemma first_nats_less (n k : nat) (H : In n (first_nats k)) : n < k.
-Proof.
-  induction k.
-  { inversion H. }
-  { inversion H. { omega. } { apply IHk in H0. omega. } }
+      red. red in HinDA. destruct HinDA as [s' [cs' [n' [Hinstr [HDAS HDACS]]]]].
+      exists s'. exists cs'. exists n'. split; auto. constructor; auto. } }
 Qed.
 
 Lemma search_completeness
       (g   : goal)
-      (CG    : consistent_goal g)
+      (CG  : consistent_goal g)
       (k   : nat)
       (HC  : closed_goal_in_context (first_nats k) g)
       (f   : repr_fun)
       (t   : trace)
-      (OP : op_sem (State (Leaf g empty_subst k)) t)
+      (OP : op_sem (State (Leaf g empty_subst init_cs k)) t)
       (HDS : [| g , f |]) :
-      exists (f' : repr_fun), (in_denotational_analog t f') /\
+      exists (f' : repr_fun), {| t , f' |} /\
                             forall (x : name), In x (first_nats k) -> gt_eq (f x) (f' x).
 Proof.
   apply in_denotational_sem_some_lev in HDS. destruct HDS as [l HDS].
-  assert (WF : well_formed_state' (Leaf g empty_subst k)).
-  { constructor.
-    { intros. good_inversion X_IN_DOM. good_inversion H. }
-    { intros. good_inversion X_IN_VRAN. destruct H as [t0 [H0 _]]. good_inversion H0. }
-    { red in HC. intros. apply first_nats_less; auto. } }
-  assert (DSS : in_denotational_sem_subst empty_subst f).
-  { red. exists f. red. intros.
-    unfold subst_repr_fun_compose. rewrite apply_empty. reflexivity. }
-  specialize (search_completeness_generalized l g CG empty_subst k WF t OP f HDS DSS).
+  assert (WF : well_formed_state' (Leaf g empty_subst init_cs k)).
+  { apply well_formed_initial_state; auto. }
+  specialize (search_completeness_generalized l g CG empty_subst init_cs k WF t OP f HDS (empty_subst_ds f) (init_condition f)).
   intro. destruct H as [f' [HinDA ff'eq]]. exists f'. split; auto.
   intros. apply ff'eq. apply first_nats_less; auto.
 Qed.
+
+End OperationalSemCompletenessAbstr.
