src/OperationalSem.v
@@ -1,16 +1,97 @@
 Require Import List.
+Import ListNotations.
 Require Import Coq.Lists.ListSet.
+Require Import Coq.Program.Equality.
+Require Import Omega.
+
 Require Import Unify.
 Require Import MiniKanrenSyntax.
 Require Import Stream.
-Require Import Omega.
-Require Import Extraction.
+Require Import DenotationalSem.
+
+
+Definition dep_pair_cs_same (A : Set)
+                            (B : A -> Set)
+                            (a : A)
+                            (b : B a)
+                            (b' : B a)
+                            (EQ : existT (fun a : A => B a) a b =
+                                  existT (fun a : A => B a) a b') :
+                            b = b'.
+Proof. inversion_sigma. subst. elim_eq_rect. reflexivity. Qed.
+
+Ltac simpl_existT_cs_same :=
+  repeat
+    (match goal with
+      [ H : existT _ ?x _ = existT _ ?x _ |- _ ] => apply dep_pair_cs_same in H; subst
+    end).
+
+
+Module Type ConstraintStoreSig.
+
+Parameter constraint_store : subst -> Set.
+
+Parameter init_cs : constraint_store empty_subst.
+
+Parameter add_constraint : forall (s : subst), constraint_store s -> term -> term -> option (constraint_store s) -> Set.
+
+Axiom add_constraint_exists :
+  forall (s : subst) (cs : constraint_store s) (t1 t2 : term),
+    {r : option (constraint_store s) & add_constraint s cs t1 t2 r}.
+
+Axiom add_constraint_unique :
+  forall (s : subst) (cs : constraint_store s) (t1 t2 : term) (r r' : option (constraint_store s)),
+    add_constraint s cs t1 t2 r -> add_constraint s cs t1 t2 r' -> r = r'.
+
+Parameter upd_cs : forall (s : subst), constraint_store s -> forall (d : subst), option (constraint_store (compose s d)) -> Set.
+
+Axiom upd_cs_exists :
+  forall (s : subst) (cs : constraint_store s) (d : subst),
+    {r : option (constraint_store (compose s d)) & upd_cs s cs d r}.
+
+Axiom upd_cs_unique :
+  forall (s : subst) (cs : constraint_store s) (d : subst) (r r' : option (constraint_store (compose s d))),
+    upd_cs s cs d r -> upd_cs s cs d r' -> r = r'.
+
+Parameter in_denotational_sem_cs : forall (s : subst), constraint_store s -> repr_fun -> Prop.
+
+Notation "[| s , cs , f |]" := (in_denotational_sem_cs s cs f) (at level 0).
+
+Axiom init_condition : forall f, [| empty_subst , init_cs , f |].
+
+Axiom add_constraint_fail_condition :
+  forall (s : subst) (cs : constraint_store s) (t1 t2 : term),
+    add_constraint s cs t1 t2 None ->
+    forall f, ~ ([| s , cs  , f |] /\ [ s , f ] /\ [| Disunify t1 t2 , f |]).
+
+Axiom add_constraint_success_condition :
+  forall (s : subst) (cs cs' : constraint_store s) (t1 t2 : term),
+    add_constraint s cs t1 t2 (Some cs') ->
+    forall f, [| s , cs' , f |] /\ [ s , f ] <->
+              [| s , cs  , f |] /\ [ s , f ] /\ [| Disunify t1 t2 , f |].
+
+Axiom upd_cs_fail_condition :
+  forall (s : subst) (cs : constraint_store s) (d : subst),
+    upd_cs s cs d None -> forall f, ~ ([| s , cs , f |] /\ [ compose s d , f ]).
+
+Axiom upd_cs_success_condition :
+  forall (s : subst) (cs : constraint_store s) (d : subst) (cs' : constraint_store (compose s d)),
+    upd_cs s cs d (Some cs') ->
+    forall f, [| compose s d , cs' , f |] /\ [ compose s d , f ] <->
+              [| s           , cs  , f |] /\ [ compose s d , f ].
+
+End ConstraintStoreSig.
+
+
+Module OperationalSemAbstr (ConstraintStore : ConstraintStoreSig).
+
+Import ConstraintStore.
 
 (* Partial state *) 
 Inductive state' : Set :=
-(* (goal, subst, first free semantic variable) *) | Leaf : goal -> subst -> nat -> state'
-(* sum of two states'                          *) | Sum  : state' -> state' -> state'
-(* product of two states'                      *) | Prod : state' -> goal   -> state'.
+| Leaf : goal -> forall (s : subst), constraint_store s -> nat -> state'
+| Sum  : state' -> state' -> state'
+| Prod : state' -> goal   -> state'.
 
 (* Complete state *)
 Inductive state : Set :=
@@ -18,8 +99,8 @@ Inductive state : Set :=
 (* a partial state   *) | State : state' -> state.
 
 Inductive is_fv_of_state' : name -> state' -> Prop :=
-| isfvst'Leaf  : forall x g s n     (X_FV_G : is_fv_of_goal x g),
-                                    is_fv_of_state' x (Leaf g s n)
+| isfvst'Leaf  : forall x g s cs n  (X_FV_G : is_fv_of_goal x g),
+                                    is_fv_of_state' x (Leaf g s cs n)
 | isfvst'SumL  : forall x st'1 st'2 (X_FV : is_fv_of_state' x st'1),
                                     is_fv_of_state' x (Sum st'1 st'2)
 | isfvst'SumR  : forall x st'1 st'2 (X_FV : is_fv_of_state' x st'2),
@@ -38,7 +119,7 @@ Inductive is_fv_of_state : name -> state -> Prop :=
 Hint Constructors is_fv_of_state.
 
 Inductive is_counter_of_state' : nat -> state' -> Prop :=
-| iscst'Leaf  : forall g s n,      is_counter_of_state' n (Leaf g s n)
+| iscst'Leaf  : forall g s cs n,   is_counter_of_state' n (Leaf g s cs n)
 | iscst'SumL  : forall n st'1 st'2 (ISC : is_counter_of_state' n st'1),
                                    is_counter_of_state' n (Sum st'1 st'2)
 | iscst'SumR  : forall n st'1 st'2 (ISC : is_counter_of_state' n st'2),
@@ -49,13 +130,14 @@ Inductive is_counter_of_state' : nat -> state' -> Prop :=
 Hint Constructors is_counter_of_state'.
 
 Inductive well_formed_state' : state' -> Set :=
-| wfLeaf : forall g s frn   (DOM_LT_COUNTER :  forall x (X_IN_DOM : in_subst_dom s x),
-                                                        x < frn)
-                            (VRAN_LT_COUNTER : forall x (X_IN_VRAN : in_subst_vran s x),
-                                                        x < frn)
-                            (FV_LT_COUNTER :   forall x (X_FV : is_fv_of_goal x g),
-                                                        x < frn),
-                            well_formed_state' (Leaf g s frn)
+| wfLeaf : forall g s cs frn
+           (DOM_LT_COUNTER  : forall x (X_IN_DOM : in_subst_dom s x), x < frn)
+           (VRAN_LT_COUNTER : forall x (X_IN_VRAN : in_subst_vran s x), x < frn)
+           (FV_LT_COUNTER   : forall x (X_FV : is_fv_of_goal x g), x < frn)
+           (DS_LT_COUNTER   : forall (f f' : repr_fun)
+                                     (REQ_ff' : forall x, x < frn -> gt_eq (f x) (f' x)),
+                                     [ s , f ] /\ [| s , cs , f |] <-> [ s , f' ] /\ [| s , cs , f' |]),
+           well_formed_state' (Leaf g s cs frn)
 | wfSum  : forall st'1 st'2 (WF_L : well_formed_state' st'1)
                             (WF_R : well_formed_state' st'2),
                             well_formed_state' (Sum st'1 st'2)
@@ -67,6 +149,37 @@ Inductive well_formed_state' : state' -> Set :=
 
 Hint Constructors well_formed_state'.
 
+Fixpoint first_nats (k : nat) : list nat :=
+  match k with
+  | 0   => []
+  | S n => n :: first_nats n
+  end.
+
+Lemma first_nats_less (n k : nat) (H : In n (first_nats k)) : n < k.
+Proof.
+  induction k.
+  { inversion H. }
+  { inversion H. { omega. } { apply IHk in H0. omega. } }
+Qed.
+
+Lemma well_formed_initial_state
+      (g   : goal)
+      (k   : nat)
+      (HC  : closed_goal_in_context (first_nats k) g) :
+      well_formed_state' (Leaf g empty_subst init_cs k).
+Proof.
+  constructor.
+  { intros. good_inversion X_IN_DOM. good_inversion H. }
+  { intros. good_inversion X_IN_VRAN. destruct H as [t0 [H0 _]]. good_inversion H0. }
+  { red in HC. intros. apply first_nats_less; auto. }
+  { intros. split; split.
+    { apply empty_subst_ds. }
+    { apply init_condition. }
+    { apply empty_subst_ds. }
+    { apply init_condition. } }
+Qed.
+
+
 Inductive well_formed_state : state -> Set :=
 | wfEmpty    : well_formed_state Stop
 | wfNonEmpty : forall st' (wfState : well_formed_state' st'),
@@ -77,44 +190,53 @@ Hint Constructors well_formed_state.
 (* Labels *)
 Inductive label : Set :=
 (* nothing                                       *) | Step   : label
-(* answer: (subst, first free semantic variable) *) | Answer : subst -> nat -> label.
+(* answer: (subst, first free semantic variable) *) | Answer : forall (s : subst), constraint_store s -> nat -> label.
 
 (* Transitions *)
 Inductive eval_step : state' -> label -> state -> Set :=
-| esFail         : forall           s    n, eval_step (Leaf Fail s n) Step Stop
-| esCut          : forall           s    n, eval_step (Leaf Cut s n)  (Answer s n) Stop                             (* cuts are ignored in interliving search *)
-| esUnifyFail    : forall t1 t2     s    n  (MGU : mgu (apply_subst s t1) (apply_subst s t2) None),
-                                            eval_step (Leaf (Unify t1 t2) s n) Step Stop
-| esUnifySuccess : forall t1 t2     s s' n  (MGU : mgu (apply_subst s t1) (apply_subst s t2) (Some s')),
-                                            eval_step (Leaf (Unify t1 t2) s n) (Answer (compose s s') n) Stop
-| esDisj         : forall g1 g2     s    n, eval_step (Leaf (Disj g1 g2) s n) Step (State (Sum (Leaf g1 s n) (Leaf g2 s n)))
-| esConj         : forall g1 g2     s    n, eval_step (Leaf (Conj g1 g2) s n) Step (State (Prod (Leaf g1 s n) g2))
-| esFresh        : forall fg        s    n, eval_step (Leaf (Fresh fg) s n)   Step (State (Leaf (fg n) s (S n)))
-| esInvoke       : forall r arg     s    n, eval_step (Leaf (Invoke r arg) s n) Step (State (Leaf (proj1_sig (MiniKanrenSyntax.Prog r) arg) s n))
-| esSumE         : forall st1 st2        l  (STEP_L : eval_step st1 l  Stop),
-                                            eval_step (Sum st1 st2) l (State st2)
-| esSumNE        : forall st1 st1' st2   l  (STEP_L : eval_step st1 l (State st1')),
-                                            eval_step (Sum st1 st2) l (State (Sum st2 st1'))
-| esProdSE       : forall st g              (STEP_L : eval_step st Step Stop),
-                                            eval_step (Prod st g) Step Stop
-| esProdAE       : forall st g s n          (STEP_L : eval_step st (Answer s n) Stop),
-                                            eval_step (Prod st g) Step (State (Leaf g s n))
-| esProdSNE      : forall st g     st'      (STEP_L : eval_step st Step (State st')),
-                                            eval_step (Prod st g) Step (State (Prod st' g))
-| esProdANE      : forall st g s n st'      (STEP_L : eval_step st (Answer s n) (State st')),
-                                            eval_step (Prod st g) Step (State (Sum (Leaf g s n) (Prod st' g))).
+| esFail         : forall           s cs       n, eval_step (Leaf Fail s cs n) Step Stop
+| esCut          : forall           s cs       n, eval_step (Leaf Cut s cs n)  (Answer s cs n) Stop                             (* cuts are ignored in interliving search *)
+| esUnifyFail    : forall t1 t2     s cs       n  (MGU : mgu (apply_subst s t1) (apply_subst s t2) None),
+                                                  eval_step (Leaf (Unify t1 t2) s cs n) Step Stop
+| esUnifyUpdFail : forall t1 t2     s cs d     n  (MGU : mgu (apply_subst s t1) (apply_subst s t2) (Some d))
+                                                  (UPD_CS : upd_cs s cs d None),
+                                                  eval_step (Leaf (Unify t1 t2) s cs n) Step Stop
+| esUnifySuccess : forall t1 t2     s cs d cs' n  (MGU : mgu (apply_subst s t1) (apply_subst s t2) (Some d))
+                                                  (UPD_CS : upd_cs s cs d (Some cs')),
+                                                  eval_step (Leaf (Unify t1 t2) s cs n) (Answer (compose s d) cs' n) Stop
+| esDisunifyFail : forall t1 t2     s cs       n  (ADD_C : add_constraint s cs t1 t2 None),
+                                                  eval_step (Leaf (Disunify t1 t2) s cs n) Step Stop
+| esDisunifySuccess : forall t1 t2     s cs cs' n  (ADD_C : add_constraint s cs t1 t2 (Some cs')),
+                                                   eval_step (Leaf (Disunify t1 t2) s cs n) (Answer s cs' n) Stop
+| esDisj         : forall g1 g2     s cs       n, eval_step (Leaf (Disj g1 g2) s cs n)   Step (State (Sum (Leaf g1 s cs n) (Leaf g2 s cs n)))
+| esConj         : forall g1 g2     s cs       n, eval_step (Leaf (Conj g1 g2) s cs n)   Step (State (Prod (Leaf g1 s cs n) g2))
+| esFresh        : forall fg        s cs       n, eval_step (Leaf (Fresh fg) s cs n)     Step (State (Leaf (fg n) s cs (S n)))
+| esInvoke       : forall r arg     s cs       n, eval_step (Leaf (Invoke r arg) s cs n) Step (State (Leaf (proj1_sig (MiniKanrenSyntax.Prog r) arg) s cs n))
+| esSumE         : forall st1 st2        l        (STEP_L : eval_step st1 l  Stop),
+                                                  eval_step (Sum st1 st2) l (State st2)
+| esSumNE        : forall st1 st1' st2   l        (STEP_L : eval_step st1 l (State st1')),
+                                                  eval_step (Sum st1 st2) l (State (Sum st2 st1'))
+| esProdSE       : forall st g                    (STEP_L : eval_step st Step Stop),
+                                                  eval_step (Prod st g) Step Stop
+| esProdAE       : forall st g s cs n             (STEP_L : eval_step st (Answer s cs n) Stop),
+                                                  eval_step (Prod st g) Step (State (Leaf g s cs n))
+| esProdSNE      : forall st g        st'         (STEP_L : eval_step st Step (State st')),
+                                                  eval_step (Prod st g) Step (State (Prod st' g))
+| esProdANE      : forall st g s cs n st'         (STEP_L : eval_step st (Answer s cs n) (State st')),
+                                                  eval_step (Prod st g) Step (State (Sum (Leaf g s cs n) (Prod st' g))).
 
 Hint Constructors eval_step.
 
 Lemma counter_in_answer
       (st' : state')
       (s : subst)
+      (cs : constraint_store s)
       (n : nat)
       (st : state)
-      (EV : eval_step st' (Answer s n) st) :
+      (EV : eval_step st' (Answer s cs n) st) :
       is_counter_of_state' n st'.
 Proof.
-  remember (Answer s n). induction EV; good_inversion Heql; auto.
+  remember (Answer s cs n). induction EV; good_inversion Heql; auto.
 Qed.
 
 Lemma counter_in_next_state
@@ -164,15 +286,16 @@ Qed.
 Lemma well_formed_subst_in_answer
       (st' : state')
       (s : subst)
+      (cs : constraint_store s)
       (n : nat)
       (st : state)
-      (EV : eval_step st' (Answer s n) st)
+      (EV : eval_step st' (Answer s cs n) st)
       (WF : well_formed_state' st') :
       (forall x, in_subst_dom s x -> x < n) /\ (forall x, in_subst_vran s x -> x < n).
 Proof.
-  remember (Answer s n). induction EV; good_inversion Heql; good_inversion WF; auto.
+  remember (Answer s cs n). induction EV; good_inversion Heql; good_inversion WF; auto.
   assert (FV_LT_N_1 : forall x, In x (fv_term (apply_subst s0 t1)) -> x < n).
-  { clear MGU s'. intros. induction t1.
+  { clear MGU H1 H3 UPD_CS. clear cs cs'. clear d. intros. induction t1.
     { simpl in H. destruct (image s0 n0) eqn:eq; auto.
       apply VRAN_LT_COUNTER. red. eauto. }
     { good_inversion H. }
@@ -184,7 +307,7 @@ Proof.
         good_inversion X_FV; auto. apply fvUnifyL. simpl.
         apply set_union_intro. right. auto. } } }
   assert (FV_LT_N_2 : forall x, In x (fv_term (apply_subst s0 t2)) -> x < n).
-  { clear MGU s'. intros. induction t2.
+  { clear MGU H1 H3 UPD_CS. clear cs cs'. clear d. intros. induction t2.
     { simpl in H. destruct (image s0 n0) eqn:eq; auto.
       apply VRAN_LT_COUNTER. red. eauto. }
     { good_inversion H. }
@@ -204,6 +327,57 @@ Proof.
     apply S'_VRAN in H. destruct H; auto. }
 Qed.
 
+Lemma well_formed_ds_in_answer
+      (st' : state')
+      (s : subst)
+      (cs : constraint_store s)
+      (n : nat)
+      (st : state)
+      (EV : eval_step st' (Answer s cs n) st)
+      (WF : well_formed_state' st')
+      (f f' : repr_fun)
+      (REQ_ff' : forall x, x < n -> gt_eq (f x) (f' x)) :
+      [ s , f ] /\ [| s , cs , f |] <-> [ s , f' ] /\ [| s , cs , f' |].
+Proof.
+  assert (AND_IFF_SPLIT : forall A B C D, (A <-> C) -> (B <-> D) -> (A /\ B <-> C /\ D)).
+  { intros. split; split; auto; destruct H1; destruct H0; destruct H; auto. }
+  remember (Answer s cs n). induction EV; good_inversion Heql; good_inversion WF; simpl_existT_cs_same; auto; specialize (DS_LT_COUNTER f f' REQ_ff').
+  { rewrite and_comm.
+    eapply iff_trans. 2: apply and_comm.
+    rewrite (upd_cs_success_condition _ _ _ _ UPD_CS).
+    rewrite (upd_cs_success_condition _ _ _ _ UPD_CS).
+    rewrite (denotational_sem_uni _ _ _ _ MGU f).
+    rewrite (denotational_sem_uni _ _ _ _ MGU f').
+    rewrite <- and_assoc. rewrite <- and_assoc.
+    apply AND_IFF_SPLIT.
+    { rewrite and_comm. rewrite DS_LT_COUNTER. apply and_comm. }
+    { split; intros.
+      { etransitivity. etransitivity.
+        2: apply H.
+        { apply apply_repr_fun_fv. intros. symmetry. apply REQ_ff'. auto. }
+        { apply apply_repr_fun_fv. intros. apply REQ_ff'. auto. } }
+      { etransitivity. etransitivity.
+        2: apply H.
+        { apply apply_repr_fun_fv. intros. apply REQ_ff'. auto. }
+        { apply apply_repr_fun_fv. intros. symmetry. apply REQ_ff'. auto. } } } }
+  { rewrite and_comm.
+    eapply iff_trans. 2: apply and_comm.
+    rewrite (add_constraint_success_condition _ _ _ _ _ ADD_C).
+    rewrite (add_constraint_success_condition _ _ _ _ _ ADD_C).
+    rewrite <- and_assoc. rewrite <- and_assoc.
+    apply AND_IFF_SPLIT.
+    { rewrite and_comm. rewrite DS_LT_COUNTER. apply and_comm. }
+    { split; intros DSG; good_inversion DSG; constructor; intro C; apply DISUNI.
+      { etransitivity. etransitivity.
+        2: apply C.
+        { apply apply_repr_fun_fv. intros. apply REQ_ff'. auto. }
+        { apply apply_repr_fun_fv. intros. symmetry. apply REQ_ff'. auto. } }
+      { etransitivity. etransitivity.
+        2: apply C.
+        { apply apply_repr_fun_fv. intros. symmetry. apply REQ_ff'. auto. }
+        { apply apply_repr_fun_fv. intros. apply REQ_ff'. auto. } } } }
+Qed.
+
 Lemma well_formedness_preservation
       (st' : state')
       (l : label)
@@ -212,11 +386,11 @@ Lemma well_formedness_preservation
       (WF : well_formed_state' st') :
       well_formed_state st.
 Proof.
-  intros. induction EV; good_inversion WF; auto.
+  intros. induction EV; good_inversion WF; simpl_existT_cs_same; auto.
   { constructor. auto. }
   { constructor. constructor; auto.
     intros. good_inversion FRN_COUNTER. subst. auto. }
-  { constructor. constructor.
+  { constructor. constructor; auto.
     1-2: intros; eapply lt_trans; eauto.
     intros. destruct (eq_nat_dec n x).
     { omega. }
@@ -226,7 +400,8 @@ Proof.
     simpl in CC. destruct CC as [CL _]. red in CL. red in CL. auto. }
   { specialize (IHEV WF_L).
     good_inversion IHEV. auto. }
-  { constructor. constructor.
+  { constructor. constructor; auto.
+    4: eapply well_formed_ds_in_answer; eauto.
     1-2: apply well_formed_subst_in_answer in EV; destruct EV; auto.
     intros. apply FV_LT_COUNTER; auto. eapply counter_in_answer; eauto. }
   { specialize (IHEV WF_L). good_inversion IHEV.
@@ -238,6 +413,7 @@ Proof.
   { specialize (IHEV WF_L). good_inversion IHEV.
     constructor. constructor.
     { constructor.
+      4: eapply well_formed_ds_in_answer; eauto.
       1-2: apply well_formed_subst_in_answer in EV; destruct EV; auto.
       intros. apply FV_LT_COUNTER; auto.
       eapply counter_in_answer; eauto. }
@@ -254,9 +430,17 @@ Lemma eval_step_exists
 Proof.
   induction st'.
   { destruct g.
-    1-2,4-7: repeat eexists; econstructor.
+    1-2,5-8: repeat eexists; econstructor.
     { assert ({r & mgu (apply_subst s t) (apply_subst s t0) r}).
       { apply mgu_exists. }
+      destruct H. destruct x.
+      { assert ({r & upd_cs s c s0 r}).
+        { apply upd_cs_exists. }
+        destruct H. destruct x.
+        all: repeat eexists; eauto. }
+      { repeat eexists; eauto. } }
+    { assert ({r & add_constraint s c t t0 r}).
+      { apply add_constraint_exists. }
       destruct H. destruct x.
       all: repeat eexists; eauto. } }
   { destruct IHst'1 as [l1 [st1 IH1]]. destruct st1.
@@ -274,15 +458,40 @@ Lemma eval_step_unique
       l1 = l2 /\ st1 = st2.
 Proof.
   revert STEP_1 STEP_2. revert l1 l2 st1 st2. induction st'.
-  { intros. destruct g; good_inversion STEP_1; good_inversion STEP_2; auto.
-    { assert (C : None = Some s').
+  { intros. destruct g; good_inversion STEP_1; good_inversion STEP_2;
+    simpl_existT_cs_same; auto.
+    { assert (C : None = Some d).
       { eapply mgu_unique; eassumption. }
       inversion C. }
-    { assert (C : None = Some s').
+    { assert (EQ : Some d = Some d0).
+      { eapply mgu_unique; eassumption. }
+      good_inversion EQ.
+      assert (C : None = Some cs').
+      { eapply upd_cs_unique; eassumption. }
+      inversion C. }
+    { assert (C : None = Some d).
       { eapply mgu_unique; eassumption. }
       inversion C. }
-    { assert (C : Some s' = Some s'0).
+    { assert (EQ : Some d = Some d0).
       { eapply mgu_unique; eassumption. }
+      good_inversion EQ.
+      assert (C : None = Some cs').
+      { eapply upd_cs_unique; eassumption. }
+      inversion C. }
+    { assert (EQ : Some d = Some d0).
+      { eapply mgu_unique; eassumption. }
+      good_inversion EQ.
+      assert (C : Some cs' = Some cs'0).
+      { eapply upd_cs_unique; eassumption. }
+      inversion C. auto. }
+    { assert (C : None = Some cs').
+      { eapply add_constraint_unique; eassumption. }
+      inversion C. }
+    { assert (C : None = Some cs').
+      { eapply add_constraint_unique; eassumption. }
+      inversion C. }
+    { assert (C : Some cs' = Some cs'0).
+      { eapply add_constraint_unique; eassumption. }
       inversion C. auto. } }
   { intros. good_inversion STEP_1; good_inversion STEP_2;
     specialize (IHst'1 _ _ _ _ STEP_L STEP_L0); inversion IHst'1;
@@ -313,7 +522,7 @@ CoFixpoint trace_from (st : state) : trace :=
     end
   end.
 
-Lemma trace_from_correct 
+Lemma trace_from_correct
       (st : state) :
       op_sem st (trace_from st).
 Proof.
@@ -329,10 +538,6 @@ Lemma op_sem_exists
 Proof.
   eexists. eapply trace_from_correct.
 Qed.
-
-Extraction Language Haskell.
-
-Extraction "extracted/interpreter.hs" op_sem_exists.
 
 Lemma op_sem_unique
       (st : state)
@@ -352,20 +557,49 @@ Proof.
     { subst. eapply CIH; eauto. } }
 Qed.
 
+Definition in_denotational_analog (t : trace) (f : repr_fun) : Prop :=
+  exists (s : subst) (cs : constraint_store s) (n : nat),
+    in_stream (Answer s cs n) t /\ [ s ,  f ] /\ [| s , cs , f |].
+
+Notation "{| t , f |}" := (in_denotational_analog t f).
+
+Inductive in_denotational_sem_state' : state' -> repr_fun -> Prop :=
+| dsst'Leaf : forall g s cs n f (DSG  : [| g , f |])
+                                (DSS  : [ s , f ])
+                                (DSCS : [| s , cs , f |]),
+                                in_denotational_sem_state' (Leaf g s cs n) f
+| dsst'SumL : forall st1' st2' f (DSST' : in_denotational_sem_state' st1' f),
+                                 in_denotational_sem_state' (Sum st1' st2') f
+| dsst'SumR : forall st1' st2' f (DSST' : in_denotational_sem_state' st2' f),
+                                 in_denotational_sem_state' (Sum st1' st2') f
+| dsst'Prod : forall st' g f (DSG : [| g , f |])
+                             (DSST' : in_denotational_sem_state' st' f),
+                             in_denotational_sem_state' (Prod st' g) f.
+
+Hint Constructors in_denotational_sem_state'.
+
+Inductive in_denotational_sem_state : state -> repr_fun -> Prop :=
+| dsstState : forall st' f (DSST' : in_denotational_sem_state' st' f),
+                           in_denotational_sem_state (State st') f.
+
+Hint Constructors in_denotational_sem_state.
+
 Lemma counter_in_trace
       (g : goal)
       (s sr : subst)
+      (cs : constraint_store s)
+      (csr : constraint_store sr)
       (n nr : nat)
       (tr : trace)
-      (OP : op_sem (State (Leaf g s n)) tr)
-      (HIn : in_stream (Answer sr nr) tr) :
+      (OP : op_sem (State (Leaf g s cs n)) tr)
+      (HIn : in_stream (Answer sr csr nr) tr) :
       n <= nr.
 Proof.
-  remember (Leaf g s n) as st'.
+  remember (Leaf g s cs n) as st'.
   assert (CNT_GE : forall n', is_counter_of_state' n' st' -> n <= n').
   { intros. subst. good_inversion H. auto. }
   clear Heqst'. revert CNT_GE OP. revert n st'.
-  remember (Answer sr nr). induction HIn; intros; subst.
+  remember (Answer sr csr nr). induction HIn; intros; subst.
   { good_inversion OP. apply counter_in_answer in EV. auto. }
   { good_inversion OP. destruct st.
     { good_inversion OP0. good_inversion HIn. }
@@ -381,14 +615,37 @@ Lemma well_formed_subst_in_trace
       (t : trace)
       (OP : op_sem st t)
       (s : subst)
+      (cs : constraint_store s)
       (n : nat)
-      (IS_ANS: in_stream (Answer s n) t) :
+      (IS_ANS: in_stream (Answer s cs n) t) :
       (forall x, in_subst_dom s x -> x < n) /\ (forall x, in_subst_vran s x -> x < n).
 Proof.
-  remember (Answer s n). revert WF OP. revert st.
+  remember (Answer s cs n). revert WF OP. revert st.
   induction IS_ANS; intros.
   { good_inversion OP. good_inversion WF.
     eapply well_formed_subst_in_answer; eauto. }
+  { good_inversion OP. good_inversion WF.
+    apply IHIS_ANS with st0; auto.
+    eapply well_formedness_preservation; eauto. }
+Qed.
+
+Lemma well_formed_ds_in_trace
+      (st : state)
+      (WF : well_formed_state st)
+      (t : trace)
+      (OP : op_sem st t)
+      (s : subst)
+      (cs : constraint_store s)
+      (n : nat)
+      (IS_ANS: in_stream (Answer s cs n) t)
+      (f f' : repr_fun)
+      (REQ_ff' : forall x, x < n -> gt_eq (f x) (f' x)) :
+      [ s , f ] /\ [| s , cs , f |] <-> [ s , f' ] /\ [| s , cs , f' |].
+Proof.
+  remember (Answer s cs n). revert WF OP. revert st.
+  induction IS_ANS; intros.
+  { good_inversion OP. good_inversion WF.
+    eapply well_formed_ds_in_answer; eauto. }
   { good_inversion OP. good_inversion WF.
     apply IHIS_ANS with st0; auto.
     eapply well_formedness_preservation; eauto. }
@@ -413,54 +670,29 @@ Proof.
   { eapply CIH; eassumption. }
 Qed.
 
-Lemma disjunction_finite_commutativity
-      (g1 g2 : goal)
-      (s : subst)
-      (n : nat)
-      (t12 t21 : trace)
-      (OP_12 : op_sem (State (Leaf (Disj g1 g2) s n)) t12)
-      (OP_21 : op_sem (State (Leaf (Disj g2 g1) s n)) t21)
-      (FIN_12 : finite t12) :
-      finite t21.
-Proof.
-  intros.
-  inversion OP_12; subst.
-  inversion EV; subst.
-  inversion FIN_12; subst.
-  inversion OP_21; subst.
-  inversion EV0; subst.
-  constructor.
-  specialize (op_sem_exists (State (Leaf g1 s n))). intro. destruct H as [t1 OP1].
-  specialize (op_sem_exists (State (Leaf g2 s n))). intro. destruct H as [t2 OP2].
-  specialize (sum_op_sem _ _ _ _ _ OP1 OP2 OP). intro.
-  specialize (sum_op_sem _ _ _ _ _ OP2 OP1 OP0). intro.
-  specialize (interleave_finite _ _ _ H). intro.
-  specialize (interleave_finite _ _ _ H0). intro.
-  apply H2. apply and_comm. apply H1. auto.
-Qed.
-
 Lemma prod_op_sem_in
       (st' : state')
       (g : goal)
       (s : subst)
+      (cs : constraint_store s)
       (n : nat)
       (t1 t2 t : trace)
       (r : label)
       (OP : op_sem (State (Prod st' g)) t)
       (OP1 : op_sem (State st') t1)
-      (OP2 : op_sem (State (Leaf g s n)) t2)
-      (IN_1 : in_stream (Answer s n) t1)
+      (OP2 : op_sem (State (Leaf g s cs n)) t2)
+      (IN_1 : in_stream (Answer s cs n) t1)
       (IN_2 : in_stream r t2) :
       in_stream r t.
 Proof.
-  revert OP OP1. revert t st'. remember (Answer s n) as r1.
+  revert OP OP1. revert t st'. remember (Answer s cs n) as r1.
   induction IN_1; intros; subst.
   { good_inversion OP1. good_inversion OP.
     good_inversion EV0; specialize (eval_step_unique _ _ _ _ _ EV STEP_L);
-    intro eqs; destruct eqs; subst; good_inversion H.
+    intro eqs; destruct eqs; subst; good_inversion H; simpl_existT_cs_same.
     { constructor. specialize (op_sem_unique _ _ _ OP2 OP1).
       intros. eapply in_equal_streams; eauto. }
-    { constructor. specialize (op_sem_exists (State (Leaf g s0 n0))).
+    { constructor. specialize (op_sem_exists (State (Leaf g s0 cs0 n0))).
       intro H. destruct H as [t3 OP3].
       specialize (op_sem_exists (State (Prod st'0 g))).
       intro H. destruct H as [t4 OP4].
@@ -474,7 +706,7 @@ Proof.
     intro eqs; destruct eqs; subst.
     1-2: good_inversion OP0; good_inversion IN_1.
     { constructor. eapply IHIN_1; eauto. }
-    { constructor. specialize (op_sem_exists (State (Leaf g s0 n0))).
+    { constructor. specialize (op_sem_exists (State (Leaf g s0 cs0 n0))).
       intro H. destruct H as [t3 OP3].
       specialize (op_sem_exists (State (Prod st'0 g))).
       intro H. destruct H as [t4 OP4].
@@ -482,3 +714,5 @@ Proof.
       intro interH. eapply interleave_in in interH.
       eapply interH. right. eapply IHIN_1; eauto. } }
 Qed.
+
+End OperationalSemAbstr.
