README.md
@@ -7,13 +7,12 @@ The folder 'src' contains the formalization of the system and all the proofs:
 - Stream.v -- (possibly infinite) streams and their properties 
 - MiniKanrenSyntax.v -- base language ('Prog' axiom here is an arbitrary correct program)
 - DenotationalSem.v -- denotational semantics
-- OperationalSem.v -- operational semantics for the interleaving search
-- OpSemSoundness.v -- soundness of the interleaving search
-- OpSemCompleteness.v -- completeness of the interleaving search
+- OperationalSem.v -- abstract constraint store definition and parametrized operational semantics
+- OpSemSoundness.v -- soundness of the interleaving search under conditions
+- OpSemCompleteness.v -- completeness of the interleaving search under conditions
+- ObviousDisequality.v -- obvious concrete implementation of constraint stores
 
 The folder 'extracted' contains reference interpreters:
 
-- interpreter.hs -- the code extracted from interleaving search semantics (from OperationalSem.v)
-- interpreter_wrapped.hs -- the code from interpreter_wrapped.hs appended with primitives for more convenient use and some tests
-- sld_interpreter.hs -- the code extracted from SLD search semantics (from OperationalSemSLD.v)
-- sld_interpreter_wrapped.hs -- the code from sld_interpreter_wrapped.hs appended with primitives for more convenient use (including the Prolog to MiniKanren translation) and some tests
+- obvious_diseq_interpreter.hs -- the code extracted from operational semantics instantiated with the obvious constraint stores implementation (from ObviousDisequality.v)
+- obvious_diseq_interpreter_wrapped.hs -- the code from obvious_diseq_interpreter.hs appended with primitives for more convenient use and some tests
